update riscv vale.i.dfy

arch/riscv/mem.i.dfy
@@ -7,119 +7,102 @@ module mem {
 
   datatype entry_t = 
     | W32(w32: uint32)
-    | B256(b256: seq<uint256>)
+    | B32(b32: seq<uint32>)
 
   type heap_t = map<int, entry_t>
 
-  function heap_b256_index_ptr(ptr: nat, i: nat): nat
+  function heap_b32_index_ptr(ptr: nat, i: nat): nat
   {
-    ptr + 32 * i
+    ptr + 4 * i
   }
 
-  predicate heap_b256_ptr_valid(heap: heap_t, base_ptr: nat)
+  predicate heap_b32_ptr_valid(heap: heap_t, base_ptr: nat)
   {
-    && ptr_admissible_256(base_ptr)
+    && ptr_admissible_32(base_ptr)
     && base_ptr in heap
-    && heap[base_ptr].B256?
-    && var len := |heap[base_ptr].b256|;
+    && heap[base_ptr].B32?
+    && var len := |heap[base_ptr].b32|;
     //  the buffer is not empty
     && len != 0
     // end of buffer is in bound
-    && ptr_admissible_256(heap_b256_index_ptr(base_ptr, len - 1))
+    && ptr_admissible_32(heap_b32_index_ptr(base_ptr, len - 1))
   }
 
-  // this holds for each uint256 in a b256 heaplet entry
-  predicate heap_256_inv(heap: heap_t, flat: flat_t, base_ptr: nat, i: nat)
-    requires heap_b256_ptr_valid(heap, base_ptr)
-    requires i < |heap[base_ptr].b256|
+  // this holds for each uint32 in a b32 heaplet entry
+  predicate heap_32_inv(heap: heap_t, flat: flat_t, base_ptr: nat, i: nat)
+    requires heap_b32_ptr_valid(heap, base_ptr)
+    requires i < |heap[base_ptr].b32|
   {
-    var ptr := heap_b256_index_ptr(base_ptr, i);
-    // ptr points to some uint256, which has 8 base words uint32
-    && flat_ptr_valid_256(flat, ptr)
-    && flat_read_256(flat, ptr) == heap[base_ptr].b256[i]
+    var ptr := heap_b32_index_ptr(base_ptr, i);
+    // ptr points to some uint32, which has 8 base words uint32
+    && flat_ptr_valid_32(flat, ptr)
+    && flat_read_32(flat, ptr) == heap[base_ptr].b32[i]
     // disjointness
     && (i != 0 ==> ptr !in heap)
-    && ptr + 4 !in heap
-    && ptr + 8 !in heap
-    && ptr + 12 !in heap
-    && ptr + 16 !in heap
-    && ptr + 20 !in heap
-    && ptr + 24 !in heap
-    && ptr + 28 !in heap
     && !in_stack_addr_range(ptr + 0)
     && ptr + 0 !in heap
-    && !in_stack_addr_range(ptr + 4)
-    && ptr + 4 !in heap
-    && !in_stack_addr_range(ptr + 8)
-    && ptr + 8 !in heap
-    && !in_stack_addr_range(ptr + 12)
-    && ptr + 12 !in heap
-    && !in_stack_addr_range(ptr + 16)
-    && ptr + 16 !in heap
-    && !in_stack_addr_range(ptr + 20)
-    && ptr + 20 !in heap
-    && !in_stack_addr_range(ptr + 24)
-    && ptr + 24 !in heap
-    && !in_stack_addr_range(ptr + 28)
-    && ptr + 28 !in heap
   }
 
-  // this holds for each b256 heaplet entry
-  predicate heap_b256_inv(heap: heap_t, flat: flat_t, base_ptr: nat)
-    requires heap_b256_ptr_valid(heap, base_ptr)
+  // this holds for each b32 heaplet entry
+  predicate heap_b32_inv(heap: heap_t, flat: flat_t, base_ptr: nat)
+    requires heap_b32_ptr_valid(heap, base_ptr)
   {
-    forall i | 0 <= i < |heap[base_ptr].b256| ::
-      heap_256_inv(heap, flat, base_ptr, i)
+    forall i | 0 <= i < |heap[base_ptr].b32| ::
+      heap_32_inv(heap, flat, base_ptr, i)
   }
 
-  function heap_b256_read(heap: heap_t, iter: b256_iter): uint256
-    requires b256_iter_safe(heap, iter)
+  function heap_b32_read(heap: heap_t, iter: b32_iter): uint32
+    requires b32_iter_safe(heap, iter)
   {
-    var buff := heap[iter.base_ptr].b256;
+    var buff := heap[iter.base_ptr].b32;
     buff[iter.index]
   }
 
-  function heap_b256_write(heap: heap_t, iter: b256_iter, value: uint256): heap_t
-    requires b256_iter_safe(heap, iter)
+  function heap_b32_write(heap: heap_t, iter: b32_iter, value: uint32): heap_t
+    requires b32_iter_safe(heap, iter)
   {
-    var buff := heap[iter.base_ptr].b256;
+    var buff := heap[iter.base_ptr].b32;
     var new_buff := buff[iter.index := value];
-    heap[iter.base_ptr := B256(new_buff)]
+    heap[iter.base_ptr := B32(new_buff)]
   }
 
 
   // iterator for buffer entries
-  datatype b256_iter = b256_iter_cons(base_ptr: nat, index: nat,
-    ptr: nat, buff: seq<uint256>)
+  datatype b32_iter = b32_iter_cons(base_ptr: nat, index: nat, buff: seq<uint32>)
+  {
+    function cur_ptr(): nat {
+      heap_b32_index_ptr(base_ptr, index)
+    }
+  }
 
-  function b256_iter_load_next(iter: b256_iter, inc: bool): b256_iter
+  function b32_iter_load_next(iter: b32_iter, inc: bool): b32_iter
   {
     iter.(index := if inc then iter.index + 1 else iter.index)
   }
 
-  function b256_iter_store_next(iter: b256_iter, value: uint256, inc: bool): b256_iter
+  function b32_iter_store_next(iter: b32_iter, value: uint32, inc: bool): b32_iter
     requires iter.index < |iter.buff|
   {
       iter.(index := if inc then iter.index + 1 else iter.index)
           .(buff := iter.buff[iter.index := value])
   }
 
-  predicate b256_iter_inv(heap: heap_t, iter: b256_iter)
+  predicate b32_iter_inv(heap: heap_t, iter: b32_iter)
   {
     var base_ptr := iter.base_ptr;
     // base_ptr points to a valid buffer
-    && heap_b256_ptr_valid(heap, base_ptr)
+    && heap_b32_ptr_valid(heap, base_ptr)
     // ptr is correct
-    && iter.ptr == heap_b256_index_ptr(base_ptr, iter.index)
+    && iter.cur_ptr() == heap_b32_index_ptr(base_ptr, iter.index)
     // the view is consistent with heap
-    && heap[base_ptr].b256 == iter.buff
+    && heap[base_ptr].b32 == iter.buff
     // the index is within bound (or at end)
     && iter.index <= |iter.buff|
   }
 
-  predicate b256_iter_safe(heap: heap_t, iter: b256_iter)
+  predicate b32_iter_safe(heap: heap_t, iter: b32_iter)
   {
-    && b256_iter_inv(heap, iter)
+    && b32_iter_inv(heap, iter)
     // tighter constraint so we can dereference
     && iter.index < |iter.buff|
   }
@@ -182,8 +165,8 @@ module mem {
     // the equivalence invariant between heaplet and memory
     predicate inv(flat: flat_t)
     {
-      && (forall base_ptr | heap_b256_ptr_valid(heap, base_ptr) ::
-        heap_b256_inv(heap, flat, base_ptr))
+      && (forall base_ptr | heap_b32_ptr_valid(heap, base_ptr) ::
+        heap_b32_inv(heap, flat, base_ptr))
       && (forall base_ptr | heap_w32_ptr_valid(heap, base_ptr) ::
         heap_w32_inv(heap, flat, base_ptr))
       && stack_inv(flat)
@@ -197,103 +180,103 @@ module mem {
 
     lemma sub_ptrs_disjoint(flat: flat_t, base1: nat, base2: nat)
       requires inv(flat)
-      requires heap_b256_ptr_valid(heap, base1)
-      requires heap_b256_ptr_valid(heap, base2)
+      requires heap_b32_ptr_valid(heap, base1)
+      requires heap_b32_ptr_valid(heap, base2)
       requires base1 != base2
       ensures forall i, j ::
-        (0 <= i < |heap[base1].b256| && 0 <= j < |heap[base2].b256|)
+        (0 <= i < |heap[base1].b32| && 0 <= j < |heap[base2].b32|)
           ==> 
-        (heap_b256_index_ptr(base1, i) != heap_b256_index_ptr(base2, j))
+        (heap_b32_index_ptr(base1, i) != heap_b32_index_ptr(base2, j))
     {
       var heap := heap;
       if exists i, j ::
-        && 0 <= i < |heap[base1].b256|
-        && 0 <= j < |heap[base2].b256|
-        && heap_b256_index_ptr(base1, i) == heap_b256_index_ptr(base2, j)
+        && 0 <= i < |heap[base1].b32|
+        && 0 <= j < |heap[base2].b32|
+        && heap_b32_index_ptr(base1, i) == heap_b32_index_ptr(base2, j)
       {
         var i, j :|
-          && 0 <= i < |heap[base1].b256|
-          && 0 <= j < |heap[base2].b256|
-          && heap_b256_index_ptr(base1, i) == heap_b256_index_ptr(base2, j);
-        assert base1 + 32 * i == base2 + 32 * j;
-        var buff1 := heap[base1].b256;
-        var buff2 := heap[base2].b256;
+          && 0 <= i < |heap[base1].b32|
+          && 0 <= j < |heap[base2].b32|
+          && heap_b32_index_ptr(base1, i) == heap_b32_index_ptr(base2, j);
+        assert base1 + 4 * i == base2 + 4 * j;
+        var buff1 := heap[base1].b32;
+        var buff2 := heap[base2].b32;
 
         if base1 > base2 {
-          assert heap_b256_inv(heap, flat, base2);
+          assert heap_b32_inv(heap, flat, base2);
           var k := j - i;
-          assert base1 == heap_b256_index_ptr(base2, k);
+          assert base1 == heap_b32_index_ptr(base2, k);
           assert 0 <= k < |buff2|;
-          assert heap_256_inv(heap, flat, base2, k);
+          assert heap_32_inv(heap, flat, base2, k);
           assert base1 !in heap;
           assert false;
         } else {
-          assert heap_b256_inv(heap, flat, base1);
+          assert heap_b32_inv(heap, flat, base1);
           var k := i - j;
-          assert base2 == heap_b256_index_ptr(base1, k);
+          assert base2 == heap_b32_index_ptr(base1, k);
           assert 0 <= k < |buff1|;
-          assert heap_256_inv(heap, flat, base1, k);
+          assert heap_32_inv(heap, flat, base1, k);
           assert base2 !in heap;
           assert false;
         }
       }
     }
 
-    lemma heap_b256_write_preserves_b256_inv(
+    lemma heap_b32_write_preserves_b32_inv(
       flat: flat_t, new_flat: flat_t,
-      iter: b256_iter, value: uint256,
+      iter: b32_iter, value: uint32,
       other_ptr: nat)
 
       requires inv(flat)
-      requires b256_iter_safe(heap, iter)
-      requires new_flat == flat_write_256(flat, iter.ptr, value)
-      requires heap_b256_ptr_valid(heap, other_ptr)
+      requires b32_iter_safe(heap, iter)
+      requires new_flat == flat_write_32(flat, iter.cur_ptr(), value)
+      requires heap_b32_ptr_valid(heap, other_ptr)
 
-      ensures heap_b256_inv(heap_b256_write(heap, iter, value),
-        flat_write_256(flat, iter.ptr, value), other_ptr)
+      ensures heap_b32_inv(heap_b32_write(heap, iter, value),
+        flat_write_32(flat, iter.cur_ptr(), value), other_ptr)
     {
-      var new_heap := heap_b256_write(heap, iter, value);
+      var new_heap := heap_b32_write(heap, iter, value);
       var base_ptr, j := iter.base_ptr, iter.index;
-      var buff := heap[other_ptr].b256;
+      var buff := heap[other_ptr].b32;
       var len := |buff|;
 
       if other_ptr == base_ptr {
         forall i | 0 <= i < len
-          ensures heap_256_inv(new_heap, new_flat, base_ptr, i)
+          ensures heap_32_inv(new_heap, new_flat, base_ptr, i)
         {
-          assert heap_256_inv(heap, flat, base_ptr, i);
+          assert heap_32_inv(heap, flat, base_ptr, i);
           if i == j {
-            value_256_from_32(value);
-            assert heap_256_inv(new_heap, new_flat, base_ptr, i);
+            value_32_from_32(value);
+            assert heap_32_inv(new_heap, new_flat, base_ptr, i);
           }
         }
       } else {
         forall i | 0 <= i < len
-          ensures heap_256_inv(new_heap, new_flat, other_ptr, i)
+          ensures heap_32_inv(new_heap, new_flat, other_ptr, i)
         {
-          assert heap_256_inv(heap, flat, other_ptr, i);
-          var ptr := heap_b256_index_ptr(other_ptr, i);
-          assert flat_ptr_valid_256(new_flat, ptr);
-          assert ptr != iter.ptr by {
+          assert heap_32_inv(heap, flat, other_ptr, i);
+          var ptr := heap_b32_index_ptr(other_ptr, i);
+          assert flat_ptr_valid_32(new_flat, ptr);
+          assert ptr != iter.cur_ptr() by {
             sub_ptrs_disjoint(flat, other_ptr, base_ptr);
           }
-          assert flat_read_256(new_flat, ptr) == buff[i];
+          assert flat_read_32(new_flat, ptr) == buff[i];
         }
       }
-      assert heap_b256_inv(heap, flat, other_ptr);
+      assert heap_b32_inv(heap, flat, other_ptr);
     }
 
-    lemma heap_b256_write_preserves_stack_inv(
+    lemma heap_b32_write_preserves_stack_inv(
       flat: flat_t, new_flat: flat_t,
-      iter: b256_iter, value: uint256)
+      iter: b32_iter, value: uint32)
 
       requires inv(flat)
-      requires b256_iter_safe(heap, iter)
-      requires new_flat == flat_write_256(flat, iter.ptr, value)
+      requires b32_iter_safe(heap, iter)
+      requires new_flat == flat_write_32(flat, iter.cur_ptr(), value)
 
-      ensures this.(heap := heap_b256_write(heap, iter, value)).stack_inv(new_flat)
+      ensures this.(heap := heap_b32_write(heap, iter, value)).stack_inv(new_flat)
     {
-      var new_heap := heap_b256_write(heap, iter, value);
+      var new_heap := heap_b32_write(heap, iter, value);
       var new_mem := this.(heap := new_heap);
   
       assert (this.(heap := new_heap)).stack_inv(new_flat) by {
@@ -304,7 +287,7 @@ module mem {
         {
           var ptr := stack_index_to_ptr(n);
           if flat[ptr] != new_flat[ptr] {
-            assert heap_256_inv(heap, flat, iter.base_ptr, iter.index);
+            assert heap_32_inv(heap, flat, iter.base_ptr, iter.index);
             assert false;
           }
         }
@@ -312,52 +295,52 @@ module mem {
       }
     }
 
-    lemma heap_b256_write_preserves_w32_inv(
+    lemma heap_b32_write_preserves_w32_inv(
       flat: flat_t, new_flat: flat_t,
-      iter: b256_iter, value: uint256, other_ptr: nat)
+      iter: b32_iter, value: uint32, other_ptr: nat)
 
       requires inv(flat)
-      requires b256_iter_safe(heap, iter)
-      requires new_flat == flat_write_256(flat, iter.ptr, value)
+      requires b32_iter_safe(heap, iter)
+      requires new_flat == flat_write_32(flat, iter.cur_ptr(), value)
       requires heap_w32_ptr_valid(heap, other_ptr)
 
-      ensures heap_w32_inv(heap_b256_write(heap, iter, value), new_flat, other_ptr)
+      ensures heap_w32_inv(heap_b32_write(heap, iter, value), new_flat, other_ptr)
     {
       if flat[other_ptr] != new_flat[other_ptr] {
-        assert heap_256_inv(heap, flat, iter.base_ptr, iter.index);
+        assert heap_32_inv(heap, flat, iter.base_ptr, iter.index);
         assert false;
       }
     }
   
-    lemma heap_b256_write_preverses_inv(
+    lemma heap_b32_write_preverses_inv(
       flat: flat_t, new_flat: flat_t,
-      iter: b256_iter, value: uint256)
+      iter: b32_iter, value: uint32)
 
       requires inv(flat)
-      requires b256_iter_safe(heap, iter)
-      requires new_flat == flat_write_256(flat, iter.ptr, value)
+      requires b32_iter_safe(heap, iter)
+      requires new_flat == flat_write_32(flat, iter.cur_ptr(), value)
 
-      ensures this.(heap := heap_b256_write(heap, iter, value)).inv(new_flat)
+      ensures this.(heap := heap_b32_write(heap, iter, value)).inv(new_flat)
     {
-      var new_heap := heap_b256_write(heap, iter, value);
+      var new_heap := heap_b32_write(heap, iter, value);
       var new_mem := this.(heap := new_heap);
 
-      forall base_ptr | heap_b256_ptr_valid(new_heap, base_ptr)
-        ensures heap_b256_inv(new_heap, new_flat, base_ptr)
+      forall base_ptr | heap_b32_ptr_valid(new_heap, base_ptr)
+        ensures heap_b32_inv(new_heap, new_flat, base_ptr)
       {
-        heap_b256_write_preserves_b256_inv(flat, new_flat, iter, value, base_ptr);
+        heap_b32_write_preserves_b32_inv(flat, new_flat, iter, value, base_ptr);
       }
       forall base_ptr | heap_w32_ptr_valid(new_heap, base_ptr)
         ensures heap_w32_inv(new_heap, new_flat, base_ptr)
       {
-        heap_b256_write_preserves_w32_inv(flat, new_flat, iter, value, base_ptr);
+        heap_b32_write_preserves_w32_inv(flat, new_flat, iter, value, base_ptr);
       }
 
-      heap_b256_write_preserves_stack_inv(
+      heap_b32_write_preserves_stack_inv(
         flat, new_flat, iter, value);
     }
 
-    lemma heap_w32_write_preserves_b256_inv(
+    lemma heap_w32_write_preserves_b32_inv(
       flat: flat_t, new_flat: flat_t,
       write_ptr: nat, value: uint32, other_ptr: nat)
 
@@ -365,17 +348,17 @@ module mem {
       requires heap_w32_ptr_valid(heap, write_ptr)
       requires new_flat == flat_write_32(flat, write_ptr, value)
 
-      requires heap_b256_ptr_valid(heap, other_ptr)
+      requires heap_b32_ptr_valid(heap, other_ptr)
 
-      ensures heap_b256_inv(heap_w32_write(heap, write_ptr, value), new_flat, other_ptr)
+      ensures heap_b32_inv(heap_w32_write(heap, write_ptr, value), new_flat, other_ptr)
     {
       var new_heap := heap_w32_write(heap, write_ptr, value);
-      assert heap_b256_inv(heap, flat, other_ptr);
-      var buff := heap[other_ptr].b256;
+      assert heap_b32_inv(heap, flat, other_ptr);
+      var buff := heap[other_ptr].b32;
       forall i | 0 <= i < |buff| 
-        ensures heap_256_inv(new_heap, new_flat, other_ptr, i)
+        ensures heap_32_inv(new_heap, new_flat, other_ptr, i)
       {
-        assert heap_256_inv(heap, flat, other_ptr, i);
+        assert heap_32_inv(heap, flat, other_ptr, i);
       }
     }
 
@@ -425,10 +408,10 @@ module mem {
     {
       var new_heap := heap_w32_write(heap, write_ptr, value);
 
-      forall base_ptr | heap_b256_ptr_valid(new_heap, base_ptr)
-        ensures heap_b256_inv(new_heap, new_flat, base_ptr)
+      forall base_ptr | heap_b32_ptr_valid(new_heap, base_ptr)
+        ensures heap_b32_inv(new_heap, new_flat, base_ptr)
       {
-        heap_w32_write_preserves_b256_inv(flat, new_flat, write_ptr, value, base_ptr);
+        heap_w32_write_preserves_b32_inv(flat, new_flat, write_ptr, value, base_ptr);
       }
       forall base_ptr | heap_w32_ptr_valid(new_heap, base_ptr)
         ensures heap_w32_inv(new_heap, new_flat, base_ptr)
@@ -438,24 +421,24 @@ module mem {
       heap_w32_write_preserves_stack_inv(flat, new_flat, value, write_ptr);
     }
 
-    lemma stack_write_preserves_b256_inv(
+    lemma stack_write_preserves_b32_inv(
       flat: flat_t, new_flat: flat_t,
       index: nat, value: uint32, base_ptr: nat)
 
       requires inv(flat)
       requires index < |stack|
       requires new_flat == flat_write_32(flat, stack_index_to_ptr(index), value)
-      requires heap_b256_ptr_valid(heap, base_ptr)
+      requires heap_b32_ptr_valid(heap, base_ptr)
   
-      ensures heap_b256_inv(heap, new_flat, base_ptr)
+      ensures heap_b32_inv(heap, new_flat, base_ptr)
     {
-      var buff := heap[base_ptr].b256;
-      var new_buff := heap[base_ptr].b256;
+      var buff := heap[base_ptr].b32;
+      var new_buff := heap[base_ptr].b32;
   
       forall i | 0 <= i < |new_buff|
-        ensures heap_256_inv(heap, new_flat, base_ptr, i) 
+        ensures heap_32_inv(heap, new_flat, base_ptr, i) 
       {
-        assert heap_256_inv(heap, flat, base_ptr, i);
+        assert heap_32_inv(heap, flat, base_ptr, i);
       }
     }
 
@@ -499,10 +482,10 @@ module mem {
 
       ensures this.(stack := stack[index := value]).inv(new_flat)
     {
-      forall base_ptr | heap_b256_ptr_valid(heap, base_ptr)
-        ensures heap_b256_inv(heap, new_flat, base_ptr)
+      forall base_ptr | heap_b32_ptr_valid(heap, base_ptr)
+        ensures heap_b32_inv(heap, new_flat, base_ptr)
       {
-        stack_write_preserves_b256_inv(flat, new_flat, index, value, base_ptr);
+        stack_write_preserves_b32_inv(flat, new_flat, index, value, base_ptr);
       }
       
       forall base_ptr | heap_w32_ptr_valid(heap, base_ptr)
@@ -531,32 +514,17 @@ module mem {
       && frames.frames_inv(get_stack(flat))
     }
 
-    function push(flat: flat_t, num_words: uint32): mem_t
-      requires inv(flat)
-      requires in_stack_addr_range(frames.sp - num_words * 4)
-    {
-      var stack := get_stack(flat);
-      this.(frames := frames.push(num_words, stack))
-    }
-
-    lemma push_preserves_inv(flat: flat_t, num_words: uint32)
-      requires push.requires(flat, num_words)
-      ensures push(flat, num_words).inv(flat)
-    {
-      frames.push_preserves_inv(num_words, get_stack(flat));
-    }
-
-    lemma heap_b256_write_preverses_inv(
-      flat: flat_t, iter: b256_iter, value: uint256)
+    lemma heap_b32_write_preverses_inv(
+      flat: flat_t, iter: b32_iter, value: uint32)
 
       requires inv(flat)
-      requires b256_iter_safe(heap, iter)
+      requires b32_iter_safe(heap, iter)
 
-      ensures this.(heap := heap_b256_write(heap, iter, value)).
-        inv(flat_write_256(flat, iter.ptr, value))
+      ensures this.(heap := heap_b32_write(heap, iter, value)).
+        inv(flat_write_32(flat, iter.cur_ptr(), value))
     {
-      var new_flat := flat_write_256(flat, iter.ptr, value);
-      as_imem(flat).heap_b256_write_preverses_inv(flat, new_flat,
+      var new_flat := flat_write_32(flat, iter.cur_ptr(), value);
+      as_imem(flat).heap_b32_write_preverses_inv(flat, new_flat,
         iter, value);
     }
 
@@ -621,5 +589,15 @@ module mem {
 
       assert as_imem(flat).(stack := stack[stack_index := value]).inv(new_flat);
     }
+  }
+
+  function push_frame(mem: mem_t, flat: flat_t, num_words: uint32): (new_mem: mem_t)
+    requires mem.inv(flat)
+    requires in_stack_addr_range(mem.frames.sp - num_words * 4)
+    ensures new_mem.inv(flat)
+  {
+    var stack := get_stack(flat);
+    mem.frames.push_preserves_inv(num_words, get_stack(flat));
+    mem.(frames := mem.frames.push(num_words, stack))
   }
 }
